src/Init/Data/Iterators/Lemmas/Consumers/Monadic/Collect.lean
@@ -18,80 +18,62 @@ public section
 namespace Std
 open Std.Iterators Std.Internal
 
-variable {α β γ : Type w} {m : Type w → Type w'} {n : Type w → Type w''}
-  {lift : ⦃δ : Type w⦄ → m δ → n δ} {f : β → n γ} {it : IterM (α := α) m β}
+variable {α β : Type w} {m : Type w → Type w'} {it : IterM (α := α) m β}
 
-private theorem IterM.DefaultConsumers.toArrayMapped.go_eq [Monad n]
-    [Iterator α m β] [LawfulMonad n] [Finite α m] {acc : Array γ} :
-    letI : MonadLift m n := ⟨lift (δ := _)⟩
-    go lift f it acc (m := m) = (do
+private theorem IterM.toArray.go_eq [Monad m]
+    [Iterator α m β] [LawfulMonad m] [Finite α m] {acc : Array β} :
+    go it acc (m := m) = (do
       match (← it.step).inflate.val with
-      | .yield it' out => go lift f it' (acc.push (← f out))
-      | .skip it' => go lift f it' acc
+      | .yield it' out => go it' (acc.push out)
+      | .skip it' => go it' acc
       | .done => return acc) := by
-  letI : MonadLift m n := ⟨lift (δ := _)⟩
-  rw [toArrayMapped.go, WellFounded.extrinsicFix₂_eq_apply]
+  rw [toArray.go, WellFounded.extrinsicFix₂_eq_apply]
   · simp only
     apply bind_congr; intro step
-    cases step.inflate using PlausibleIterStep.casesOn
-    · apply bind_congr; intro fx
-      simp [go]
-    · simp [go]
-    · simp
+    cases step.inflate using PlausibleIterStep.casesOn <;> simp [go]
   · simp only [show (IterM.finitelyManySteps! = IterM.finitelyManySteps) by rfl]
     apply InvImage.wf
     exact WellFoundedRelation.wf
 
-private theorem IterM.DefaultConsumers.toArrayMapped.go.aux₁ [Monad n] [LawfulMonad n]
-    [Iterator α m β] [Finite α m] {b : γ} {bs : Array γ} :
-    IterM.DefaultConsumers.toArrayMapped.go lift f it (#[b] ++ bs) (m := m) =
-      (#[b] ++ ·) <$> IterM.DefaultConsumers.toArrayMapped.go lift f it bs (m := m) := by
+private theorem IterM.toArray.go.aux₁ [Monad m] [LawfulMonad m]
+    [Iterator α m β] [Finite α m] {b : β} {bs : Array β} :
+    IterM.toArray.go it (#[b] ++ bs) (m := m) =
+      (#[b] ++ ·) <$> IterM.toArray.go it bs (m := m) := by
   induction it using IterM.inductSteps generalizing bs with | step it ihy ihs
   rw [go_eq, map_eq_pure_bind, go_eq, bind_assoc]
   apply bind_congr; intro step
   cases step.inflate using PlausibleIterStep.casesOn <;> simp (discharger := assumption) [ihy, ihs]
 
-private theorem IterM.DefaultConsumers.toArrayMapped.go.aux₂ [Monad n] [LawfulMonad n]
-    [Iterator α m β] [Finite α m] {acc : Array γ} :
-    IterM.DefaultConsumers.toArrayMapped.go lift f it acc (m := m) =
-      (acc ++ ·) <$> IterM.DefaultConsumers.toArrayMapped lift f it (m := m) := by
+private theorem IterM.toArray.go.aux₂ [Monad m] [LawfulMonad m]
+    [Iterator α m β] [Finite α m] {acc : Array β} :
+    IterM.toArray.go it acc (m := m) =
+      (acc ++ ·) <$> it.toArray := by
   rw [← Array.toArray_toList (xs := acc)]
   generalize acc.toList = acc
   induction acc with
-  | nil => simp [toArrayMapped]
+  | nil => simp [toArray]
   | cons x xs ih =>
-    rw [List.toArray_cons, IterM.DefaultConsumers.toArrayMapped.go.aux₁, ih]
+    rw [List.toArray_cons, IterM.toArray.go.aux₁, ih]
     simp only [Functor.map_map, Array.append_assoc]
 
-theorem IterM.DefaultConsumers.toArrayMapped_eq_match_step [Monad n] [LawfulMonad n]
+theorem IterM.toArray_eq_match_step [Monad m] [LawfulMonad m]
     [Iterator α m β] [Finite α m] :
-    IterM.DefaultConsumers.toArrayMapped lift f it (m := m) = letI : MonadLift m n := ⟨lift (δ := _)⟩; (do
+    IterM.toArray it (m := m) = (do
       match (← it.step).inflate.val with
-      | .yield it' out =>
-        return #[← f out] ++ (← IterM.DefaultConsumers.toArrayMapped lift f it' (m := m))
-      | .skip it' => IterM.DefaultConsumers.toArrayMapped lift f it' (m := m)
+      | .yield it' out => return #[out] ++ (← it'.toArray)
+      | .skip it' => it'.toArray
       | .done => return #[]) := by
-  rw [IterM.DefaultConsumers.toArrayMapped, IterM.DefaultConsumers.toArrayMapped.go_eq]
+  rw [IterM.toArray, IterM.toArray.go_eq]
   apply bind_congr
   intro step
   cases step.inflate using PlausibleIterStep.casesOn <;>
-    simp [IterM.DefaultConsumers.toArrayMapped.go.aux₂]
+    simp [IterM.toArray.go.aux₂]
 
 @[simp]
 theorem IterM.toArray_ensureTermination [Monad m] [Iterator α m β] [Finite α m]
     {it : IterM (α := α) m β} :
     it.ensureTermination.toArray = it.toArray :=
   (rfl)
-
-theorem IterM.toArray_eq_match_step [Monad m] [LawfulMonad m] [Iterator α m β] [Finite α m] :
-    it.toArray = (do
-      match (← it.step).inflate.val with
-      | .yield it' out => return #[out] ++ (← it'.toArray)
-      | .skip it' => it'.toArray
-      | .done => return #[]) := by
-  simp only [IterM.toArray]
-  rw [IterM.DefaultConsumers.toArrayMapped_eq_match_step]
-  simp [bind_pure_comp, pure_bind]
 
 theorem IterM.toArray_ensureTermination_eq_match_step [Monad m] [LawfulMonad m] [Iterator α m β]
     [Finite α m] :
